More progress on the interface; need to discuss rw index; need to provide values for labels in spec

providers/quic/Impl.QUIC.fsti
@@ -38,8 +38,8 @@ let lbytes = Spec.QUIC.lbytes
 /// functions, and to give easier projectors (ADL, JP).
 type index = {
   role: role;
-  hash_alg: Spec.Hash.Definitions.hash_alg;
-  aead_alg: Spec.AEAD.alg;
+  hash_alg: Spec.QUIC.ha;
+  aead_alg: Spec.QUIC.ea
 }
 
 /// Boilerplate
@@ -86,10 +86,30 @@ val invariant_loc_in_footprint
 /// Attempting a new convention to distinguish ghost accessors from stateful
 /// functions: a ``g_`` prefix.
 
-val g_aead_key: #i:index -> (s: state_s i) -> (h: HS.mem) -> Spec.AEAD.kv i.aead_alg
-val g_static_iv: #i:index -> (s: state_s i) -> (h: HS.mem) -> lbytes 12
-val g_counter: #i:index -> (s: state_s i) -> (h: HS.mem) -> Spec.QUIC.nat62
-val g_hash: #i:index -> (s: state_s i) -> (h: HS.mem) -> Spec.Hash.Definitions.bytes_hash i.hash_alg
+val g_aead_key: #i:index -> (s: state_s i) -> (h: HS.mem) -> GTot (Spec.AEAD.kv i.aead_alg)
+val g_static_iv: #i:index -> (s: state_s i) -> (h: HS.mem) -> GTot (lbytes 12)
+val g_hash: #i:index -> (s: state_s i) -> (h: HS.mem) ->
+  GTot (Spec.Hash.Definitions.bytes_hash i.hash_alg)
+
+#push-options "--max_ifuel 1" // inversion on hash_alg
+let hash_is_keysized #i (s: state_s i) (h: HS.mem): Lemma
+  (ensures (Spec.QUIC.keysized i.hash_alg (S.length (g_hash s h))))
+  [ SMTPat (g_hash s h) ]
+=
+  assert_norm (512 < pow2 61);
+  assert_norm (512 < pow2 125)
+#pop-options
+
+/// Note that this one does *NOT* take the memory as an argument. (This is
+/// because the initial packet number is erased in the concrete state.) Callers
+/// should be able to derive, from this, that the initial packet number remains
+/// the same.
+val g_initial_packet_number: #i:index -> (s: state_s i) -> GTot Spec.QUIC.nat62
+
+val g_packet_number: #i:index -> (s: state_s i) -> (h: HS.mem) ->
+  GTot (pn:Spec.QUIC.nat62{
+    pn >= g_initial_packet_number s
+  })
 
 /// Preserving all the ghost accessors via a single framing lemma only works
 /// because we don't do stack allocation. See comments in
@@ -104,7 +124,7 @@ val frame_invariant: #i:index -> l:B.loc -> s:state i -> h0:HS.mem -> h1:HS.mem 
     footprint h0 s == footprint h1 s /\
     g_aead_key (B.deref h0 s) == g_aead_key (B.deref h1 s) /\
     g_static_iv (B.deref h0 s) == g_static_iv (B.deref h1 s) /\
-    g_counter (B.deref h0 s) == g_counter (B.deref h1 s) /\
+    g_packet_number (B.deref h0 s) == g_packet_number (B.deref h1 s) /\
     g_hash (B.deref h0 s) == g_hash (B.deref h1 s)
     ))
   // Assertion failure: unexpected pattern term
@@ -115,6 +135,58 @@ val frame_invariant: #i:index -> l:B.loc -> s:state i -> h0:HS.mem -> h1:HS.mem 
     [ SMTPat (g_static_iv (B.deref h1 s)) ];
     [ SMTPat (g_counter (B.deref h1 s)) ]
   ]]*)
+
+/// Low-level types used in this API
+/// --------------------------------
+
+type u2 = n:U8.t{U8.v n < 4}
+type u4 = n:U8.t{U8.v n < 16}
+type u62 = n:UInt64.t{UInt64.v n < pow2 62}
+
+let add3 (k:u4) : n:U8.t{U8.v n <= 18} = if k = 0uy then 0uy else U8.(k +^ 3uy)
+
+/// Information stored in a QUIC header. This is a Low* type passed by value --
+/// it's a little expensive. Consider passing it by reference?
+///
+/// Note that we try to follow the convention of buffer arguments followed by
+/// their lengths.
+noeq type header =
+  | Short:
+    spin: bool ->
+    phase: bool ->
+    cid: B.buffer U8.t ->
+    cid_len: U8.t{
+      let l = U8.v cid_len in
+      (l == 0 \/ (4 <= l /\ l <= 18)) /\
+      U8.v cid_len == B.length cid
+    } ->
+    header
+
+  | Long:
+    typ: u2 ->
+    version: U32.t ->
+    dcid: B.buffer U8.t ->
+    dcil: u4 { B.length dcid == U8.v (add3 dcil) } ->
+    scid: B.buffer U8.t ->
+    scil: u4 { B.length scid == U8.v (add3 scil) } ->
+    plain_len: U32.t{U32.v plain_len < Spec.QUIC.max_cipher_length} ->
+    header
+
+let _: squash (inversion header) = allow_inversion header
+
+let header_live (h: header) (m: HS.mem) =
+  match h with
+  | Short _ _ cid _ -> m `B.live` cid
+  | Long _ _ dcid _ scid _ _ -> m `B.live` dcid /\ m `B.live` scid
+
+let g_header (h: header) (m: HS.mem): GTot Spec.QUIC.header =
+  match h with
+  | Short spin phase cid cid_len ->
+      Spec.QUIC.Short spin phase (B.as_seq m cid)
+  | Long typ version dcid dcil scid scil plain_len ->
+      Spec.QUIC.Long (U8.v typ) (U32.v version) (U8.v dcil) (U8.v scil)
+      (B.as_seq m dcid) (B.as_seq m scid) (U32.v plain_len)
+
 
 /// Actual stateful API
 /// -------------------
@@ -135,10 +207,14 @@ val hash_alg_of_state (i: G.erased index) (s: state (G.reveal i)): Stack hash_al
     a == (G.reveal i).hash_alg /\
     h0 == h1))
 
-// TODO: move to spec
-val label_key : Spec.QUIC.lbytes 3
-val label_iv : Spec.QUIC.lbytes 2
-val label_hp : Spec.QUIC.lbytes 2
+val packet_number_of_state (i: G.erased index) (s: state (G.reveal i)): Stack U64.t
+  (requires fun h0 -> invariant h0 s)
+  (ensures fun h0 ctr h1 ->
+    U64.v ctr == g_packet_number (B.deref h0 s) h0 /\
+    h0 == h1)
+
+let incrementable (#i: index) (s: state i) (h: HS.mem) =
+  g_packet_number (B.deref h s) h + 1 < pow2 62
 
 val encrypt: #i:G.erased index -> (
   let i = G.reveal i in
@@ -156,25 +232,32 @@ val encrypt: #i:G.erased index -> (
     (requires fun h0 ->
       // Memory & preservation
       B.live h0 plain /\ B.live h0 dst /\
-      B.disjoint plain dst /\ // JP: probably needed, along with many others
+      header_live h h0 /\
+      B.disjoint plain dst /\ // JP: probably needed, along with many others -- TBD as we go
+
       invariant h0 s /\
 
-      i.role = Writer /\
-      // TODO: same length condition as in QuicCrypto.fsti
+      i.role = Writer /\ // JP: why does the role matter at all here?
+      incrementable s h0 /\ (
 
-      True)
+      let clen = U32.v plain_len + Spec.AEAD.tag_length i.aead_alg in
+      let len = clen + Spec.QUIC.header_len (g_header h h0) (U8.v pn_len) in
+      (Long? h ==> U32.v (Long?.plain_len h) = clen) /\
+      B.length dst == len
+    ))
     (ensures fun h0 r h1 ->
       // Memory & preservation
       B.modifies (footprint h0 s) h0 h1 /\
       invariant h1 s /\
-      footprint h1 s == footprint h0 s /\ (
+      footprint h1 s == footprint h0 s /\ ( // JP: probably footprint_s here? for precision?
 
       // Functional correctness
-      let s0 = g_hash (B.deref h0 s) in
-      let k = Spec.QUIC.derive_secret i.hash_alg s0 label_key (Spec.AEAD.key_length a.ea) in
-      let iv = Spec.QUIC.derive_secret i.hash_alg s0 label_iv 12 in
-      let pne = Spec.QUIC.derive_secret i.hash_alg s0 label_hp (Spec.QUIC.ae_keysize a.ea) in
-      let plain: Spec.QUIC.pbytes = B.as_seq h0 plain in
-      let packet: Spec.QUIC.packet = B.as_seq h1 out in
-      let ctr = pnT s Writer h0 in
-      packet == Spec.QUIC.encrypt a.ea k iv pne (U8.v pn_len) ctr (spec_header h h0) plain)))
+      let s0 = g_hash (B.deref h0 s) h0 in
+      let open Spec.QUIC in
+      let k = derive_secret i.hash_alg s0 label_key (Spec.AEAD.key_length i.aead_alg) in
+      let iv = derive_secret i.hash_alg s0 label_iv 12 in
+      let pne = derive_secret i.hash_alg s0 label_hp (ae_keysize i.aead_alg) in
+      let plain: pbytes = B.as_seq h0 plain in
+      let packet: packet = B.as_seq h1 dst in
+      let ctr = g_packet_number (B.deref h0 s) h0 in
+      packet == Spec.QUIC.encrypt i.aead_alg k iv pne (U8.v pn_len) ctr (g_header h h0) plain)))
